examples/dsls/mini_steel/Pulse.Soundness.VPropEquiv.fst
@@ -109,7 +109,7 @@ let vprop_equiv_ext_type : R.term =
   let open R in
   let v_typ = pack_ln (Tv_FVar  (pack_fv vprop_lid)) in
   let mk_bv index = pack_ln (Tv_BVar (pack_bv {
-    bv_ppname = "_";
+    bv_ppname = Sealed.seal "_";
     bv_index = index;
     bv_sort = vprop_tm;
   })) in
@@ -144,16 +144,10 @@ let rec vprop_equiv_soundness (#f:stt_env) (#g:env) (#v0 #v1:pure_term)
           RT.typing (extend_env_l f g) pf (stt_vprop_equiv (elab_pure v0) (elab_pure v1)))
          (decreases eq)
   = match eq with
-    | VE_Refl _ _ _ ->
-      assert (RT.term_no_pp (stt_vprop_equiv (elab_pure v0) (elab_pure v0)) ==
-              stt_vprop_equiv (RT.term_no_pp (elab_pure v0)) (RT.term_no_pp (elab_pure v0)));
-      elab_pure_eq_tm v0 v1;
-      assert (RT.alpha_equivalent_terms (stt_vprop_equiv (elab_pure v0) (elab_pure v0))
-                                        (stt_vprop_equiv (elab_pure v0) (elab_pure v1)));
+    | VE_Refl _ _ ->
       let d = tot_typing_soundness d in
-      let (| pf, d |) = inst_vprop_equiv_refl d in
-      (| pf, RT.T_AlphaRenaming _ _ _ d _ _ _ |)
-
+      inst_vprop_equiv_refl d
+    
     | VE_Sym g _v1 _v0 eq' ->
       let fwd, _ = vprop_equiv_typing _ _ _ _ eq in
       let d' = fwd d in
